track Cat as list of items

regex-new.dfy
@@ -1,43 +1,24 @@
 datatype Bit = B0 | B1
-datatype Reg = Cat(first: Reg, second: Reg) | Lit(Bit) | OnlyEmpty | Plus(rep: Reg) | Alt(first: Reg, second: Reg) | Never | Any
+datatype Reg = Cat(items: seq<Reg>) | Lit(Bit)| Plus(rep: Reg) | Alt(first: Reg, second: Reg) | Never | Any
 
 function method cat(a: Reg, b: Reg): Reg {
   match (a, b) {
-    case (Never, b) => Never
-    case (a, Never) => Never
-    case (OnlyEmpty, b) => b
-    case (a, OnlyEmpty) => a
+    // case (Never, b) => Never
+    // case (a, Never) => Never
     case (Any, Any) => Any
-    case _ => Cat(a, b)
+    case _ => Cat([a, b])
   }
 }
 
 lemma cat_works(a: Reg, b: Reg)
-ensures forall tape: seq<Bit> | matches(tape, Cat(a, b)) :: matches(tape, cat(a, b))
+ensures forall tape: seq<Bit> | matches(tape, Cat([a, b])) :: matches(tape, cat(a, b))
 {
   match (a, b) {
-    case (Never, b) => {
-      //
-    }
-    case (a, Never) => {
-      //
-    }
-    case (OnlyEmpty, b) => {
-      //
-    }
     case (Any, Any) => {
       // ...
     }
-    case (a, OnlyEmpty) => {
-      forall tape: seq<Bit> | matches(tape, Cat(a, b)) ensures matches(tape, cat(a, b)) {
-        var n :| 0 <= n <= |tape| && matches(tape[..n], a) && matches(tape[n..], b);
-        assert n == |tape|;
-        assert tape[..n] == tape;
-        assert matches(tape, a);
-      }
-    }
     case _ => {
-      assert cat(a, b) == Cat(a, b);
+      assert cat(a, b) == Cat([a, b]);
     }
   }
 }
@@ -61,13 +42,16 @@ ensures forall t: seq<Bit> :: matches(t, Alt(a, b)) ==> matches(t, alt(a, b))
 
 }
 
+function reg_sum_size(rs: seq<Reg>): nat {
+  if rs == [] then 1 else reg_size(rs[0]) + 1 + reg_sum_size(rs[1..])
+}
+
 function reg_size(r: Reg): nat {
   match r {
   case Never => 1
-  case Cat(a, b) => 1 + reg_size(a) + reg_size(b)
+  case Cat(list) => reg_sum_size(list)
   case Alt(a, b) => 1 + reg_size(a) + reg_size(b)
   case Lit(_) => 1
-  case OnlyEmpty => 1
   case Plus(r) => 1 + reg_size(r)
   case Any => 1
   }
@@ -78,23 +62,42 @@ decreases reg_size(r), |s|
 {
   match r {
   case Never => false
-  case Cat(a, b) => exists n :: 0 <= n <= |s| && matches(s[..n], a) && matches(s[n..], b)
+  case Cat(list) => if list == []
+    then s == []
+    else
+      assert reg_size(list[0]) < reg_size(r);
+      assert reg_size(Cat(list[1..])) < reg_size(r);
+      exists n :: 0 <= n <= |s| && matches(s[..n], list[0]) && matches(s[n..], Cat(list[1..]))
   case Alt(a, b) => matches(s, a) || matches(s, b)
-  case OnlyEmpty => s == []
   case Lit(b) => s == [b]
   case Plus(r) => matches(s, r) || exists n :: 1 <= n <= |s| && matches(s[..n], r) && matches(s[n..], Plus(r))
   case Any => true
   }
 }
 
+lemma catenating_matches_single(t: seq<Bit>, r: Reg)
+requires matches(t, r)
+ensures matches(t, Cat([r]))
+{
+  var n := |t|;
+  assert t == t[..n];
+  assert matches(t[..n], r);
+  assert matches(t[n..], Cat([]));
+}
+
 lemma catenating_matches_cat(ta: seq<Bit>, tb: seq<Bit>, a: Reg, b: Reg)
 requires matches(ta, a)
 requires matches(tb, b)
-ensures matches(ta + tb, Cat(a, b))
+ensures matches(ta + tb, Cat([a, b]))
 {
   var t := ta + tb;
   var n := |ta|;
   assert matches(t[..n], a);
+  var trail := t[n..];
+  assert matches(trail, b);
+  catenating_matches_single(trail, b);
+  assert matches(trail, Cat([b]));
+  assert matches(ta + tb, Cat([a, b]));
 }
 
 datatype Deriv = Deriv(can_be_empty: bool, after_0: Reg, after_1: Reg)
@@ -116,11 +119,8 @@ ensures forall t: seq<Bit> | t != [] && t[0] == B1 && matches(t, r) :: matches(t
         after_1 := Any
       );
     }
-    case OnlyEmpty => {
-      return Deriv(can_be_empty := true, after_0 := Never, after_1 := Never);
-    }
     case Lit(b) => {
-      return Deriv(can_be_empty := false, after_0 := if b == B0 then OnlyEmpty else Never, after_1 := if b == B1 then OnlyEmpty else Never);
+      return Deriv(can_be_empty := false, after_0 := if b == B0 then Cat([]) else Never, after_1 := if b == B1 then Cat([]) else Never);
     }
     case Plus(rep) => {
       assert reg_size(rep) < reg_size(r);
@@ -144,7 +144,7 @@ ensures forall t: seq<Bit> | t != [] && t[0] == B1 && matches(t, r) :: matches(t
           assert matches(t_left[1..], drep.after_0);
           assert matches(t_right, Plus(rep));
           catenating_matches_cat(t_left[1..], t_right, drep.after_0, Plus(rep));
-          assert matches(t_left[1..] + t_right, Cat(drep.after_0, Plus(rep)));
+          assert matches(t_left[1..] + t_right, Cat([drep.after_0, Plus(rep)]));
           assert t_left[1..] + t_right == t[1..];
           assert matches(t[1..], result.after_0);
         }
@@ -162,7 +162,7 @@ ensures forall t: seq<Bit> | t != [] && t[0] == B1 && matches(t, r) :: matches(t
           assert matches(t_left[1..], drep.after_1);
           assert matches(t_right, Plus(rep));
           catenating_matches_cat(t_left[1..], t_right, drep.after_1, Plus(rep));
-          assert matches(t_left[1..] + t_right, Cat(drep.after_1, Plus(rep)));
+          assert matches(t_left[1..] + t_right, Cat([drep.after_1, Plus(rep)]));
           assert t_left[1..] + t_right == t[1..];
           assert matches(t[1..], result.after_1);
         }
@@ -178,8 +178,20 @@ ensures forall t: seq<Bit> | t != [] && t[0] == B1 && matches(t, r) :: matches(t
         after_1 := Alt(da.after_1, db.after_1)
       );
     }
-    case Cat(a, b) => {
+    case Cat(list) => {
+      if list == [] {
+        return Deriv(
+          can_be_empty := true,
+          after_0 := Never,
+          after_1 := Never
+        );
+      }
+
+      var a := list[0];
+      var b := Cat(list[1..]);
+      assert reg_size(a) < reg_size(r);
       var da := deriv_of(a);
+      assert reg_size(b) < reg_size(r);
       var db := deriv_of(b);
       if da.can_be_empty {
         result := Deriv(
@@ -208,6 +220,7 @@ ensures forall t: seq<Bit> | t != [] && t[0] == B1 && matches(t, r) :: matches(t
           var n :| 0 <= n <= |t| && matches(t[..n], a) && matches(t[n..], b);
           if n == 0 {
             // Automatic.
+            assert matches(t[1..], result.after_0);
           } else {
             assert n >= 1;
             var t_tail := t[1..];
@@ -215,6 +228,11 @@ ensures forall t: seq<Bit> | t != [] && t[0] == B1 && matches(t, r) :: matches(t
             assert t_tail[n-1..] == t[n..];
             assert matches(t_tail[..n-1], da.after_0);
             assert matches(t_tail[n-1..], b);
+            cat_works(da.after_0, b);
+            catenating_matches_cat(t_tail[..n-1], t_tail[n-1..], da.after_0, b);
+            assert t_tail[..n-1] + t_tail[n-1..] == t_tail;
+            assert matches(t[1..], cat(da.after_0, b));
+            assert matches(t[1..], result.after_0);
           }
         }
         forall t: seq<Bit> | t != [] && t[0] == B1 && matches(t, r)
@@ -222,6 +240,7 @@ ensures forall t: seq<Bit> | t != [] && t[0] == B1 && matches(t, r) :: matches(t
           var n :| 0 <= n <= |t| && matches(t[..n], a) && matches(t[n..], b);
           if n == 0 {
             // Automatic.
+            assert matches(t[1..], result.after_1);
           } else {
             assert n >= 1;
             var t_tail := t[1..];
@@ -229,6 +248,11 @@ ensures forall t: seq<Bit> | t != [] && t[0] == B1 && matches(t, r) :: matches(t
             assert t_tail[n-1..] == t[n..];
             assert matches(t_tail[..n-1], da.after_1);
             assert matches(t_tail[n-1..], b);
+            cat_works(da.after_1, b);
+            catenating_matches_cat(t_tail[..n-1], t_tail[n-1..], da.after_1, b);
+            assert t_tail[..n-1] + t_tail[n-1..] == t_tail;
+            assert matches(t[1..], cat(da.after_1, b));
+            assert matches(t[1..], result.after_1);
           }
         }
         return result;
@@ -249,6 +273,9 @@ ensures forall t: seq<Bit> | t != [] && t[0] == B1 && matches(t, r) :: matches(t
           assert t_tail[n-1..] == t[n..];
           assert matches(t_tail[..n-1], da.after_0);
           assert matches(t_tail[n-1..], b);
+          assert t_tail[..n-1] + t_tail[n-1..] == t_tail;
+          catenating_matches_cat(t_tail[..n-1], t_tail[n-1..], da.after_0, b);
+          assert matches(t[1..], result.after_0);
         }
         forall t: seq<Bit> | t != [] && t[0] == B1 && matches(t, r)
         ensures matches(t[1..], result.after_1) {
@@ -258,6 +285,8 @@ ensures forall t: seq<Bit> | t != [] && t[0] == B1 && matches(t, r) :: matches(t
           assert t_tail[..n-1] == t[1..n];
           assert t_tail[n-1..] == t[n..];
           assert matches(t_tail[..n-1], da.after_1);
+          assert t_tail[..n-1] + t_tail[n-1..] == t_tail;
+          catenating_matches_cat(t_tail[..n-1], t_tail[n-1..], da.after_1, b);
           assert matches(t_tail[n-1..], b);
         }
         return result;
